1. Prove each of the following. Indicate which proof method you are using and show your work.
  A. Show that the square root of 2 is irrational:
    (CONTRADICTION) Suppose that the sqrt(2) is rational and can be written as two integers (p and q). We would have to assume that 
    p and q have no common factors. 
      - If we were square both side we get 2 = p^2/q^2
      - p^2 = 2q^2
      - p^2 is even.
      - p itself has to be even
      - p^2 is divisible by four.
      - therefore q is even
      - p and q are both even 
      - this contradicts to our assumption that they have not common factors. 
      - sqrt(2) can't be rational.

  B. If n = 25, 100, or 169, then n is a perfect square and is the sum of two perfect squares:
    (EXHAUSTIVE) 
    If n = 25:
      - sqrt(25) = 5
      - 16 + 9 = 25
      - sqrt(16) = 4 && sqrt(9) = 3
    If n = 100:
      - sqrt(100) = 10
      - 64 + 36 = 100
      - sqrt(64) = 8 && sqrt(36) = 6
    If n = 169:
      - sqrt(169) = 13
      - 144 + 25 = 169
      - sqrt(144) = 12 && sqrt(25) = 5
  C. The sum of two odd integers is even. Hint: By definition, even integers can be expressed as 2n, 
  thus odd integers can be expressed as 2n + 1:
    (DIRECT PROOF)
    Odd integer = 2n +- 1
    Even integer = 2n
      - Sum of two odd integers = (2n + 1) + (2n + 1)
                             = 4n + 1
                             = 2(2n + 1)
      - Let k be (2n + 1)
      - 2K
      - 2K by definition is even.
  D. The sum of an even integer and it's square is even:
    (DIRECT PROOF)
    Even integer = 2n
    Even integer and its square = (2n)^2 = 4n^2
      - 2n + (4n^2)
      - 2n(1 + 2n)
      - let K = (1 + 2n)
      - 2nk
      - let m = nk
      - 2m
      - 2m is even by definition
  E. If n squared is odd, then n is odd:
    (CONTRAPOSITION) If n squared is even, then n is even.
    n is an even integer: n = 2k
    n is squared is even: (2k)^2 => 4k^2 => 2(2k^2)
      - let p = 2k^2
      - 2p is even    

2. Part 2:
  A. Prove by induction that 1 + 5 + 9 + ... + (4n-3) = n(2n-1):
    Base Case: Assume that n = 1.
      - 1(2(1)-1) = 1
      - 1(1) = 1
      - 1 = 1 Base Case is true!
    Assume true for K
      - Show true for k 
      - 1 + 5 + 9 + ... + (4k-3) + (4(k + 1) - 3) = (k + 1)(2(k + 1) - 1)
      - 1 + 5 + 9 + ... + (4k-3) + (4k + 1)       = (k + 1)(2k + 1) 
    If we assume that it is true for (1 + 5 + 9 + ... + (4k-3) the we can plug it in
      - k(2k - 1) + (4k + 1) = (k + 1)(2k + 1)  
      - 2k^2 - k + 4k + 1 = 2k^2 + k + 2k + 1
      - 2k^2 + 3k + 1 = 2k^2 + 3k + 1
    We have proven for n and n + 1
  B. Prove that for any positive integer number n, n^3 + 2n is divisible by 3
    n > 0
    Show: 1, 2, 3, ... n => n^3 + 2n = 3m
    Base Case: Assume that n = 1
      - 1^3 + 2(1)
      - 1 + 2
      - 3 is divisable by 3
    Assume true for k
      - Show true for (k + 1)
      - 1, 2 , 3, ... , k, (k + 1) => (k + 1)^3 + 2(k + 1)
      - k^3 + 3k^2 + 3k + 1 + 2k + 2
      - (k^3 + 2k) + 3k^2 + 3k + 3
      - 3m + 3k^2 + 3k + 3
      - 3(m + k^2 +k + 1)
    By multipling it by three we know it is divisable by three. 
  C. Prove that for n >= 1, 9^n âˆ’ 1 is divisible by 8 for all non-negative integers 
   Hint: 4^(3+1) = 4 * 4^3 Hint: If 9^n - 1 = 8m, then 9^n = 8m + 1
   Base Case: Assume that n = 1
    - 9^1 - 1
    - 9 -1
    - 8 is divisible by 8
   Show 1, 2, 3, ... , n => 9^n - 1 * 8m
    - 1, 2, 3, ... , n, n + 1 => 9^(n + 1) - 1 = 8m
    - 9^n * ( -1
    - (8m + 1) * 9 -1
    - 72m + 9
    - 8(9m + 1)
   It is divisible by 8!
